Update the tests for External

tests/lean/External/Types.lean
@@ -6,4 +6,10 @@ open Primitives
 
 namespace external
 
+/- Trait declaration: [core::marker::Copy]
+   Source: '/rustc/d59363ad0b6391b7fc5bbb02c9ccf9300eef3753/library/core/src/marker.rs', lines 450:0-450:21
+   Name pattern: core::marker::Copy -/
+structure core.marker.Copy (Self : Type) where
+  cloneCloneInst : core.clone.Clone Self
+
 end external
