tests/lean/External/TypesExternal.lean
@@ -1,11 +1,20 @@
 -- [external]: external types.
 import Base
-open Primitives
+open Lean Primitives
 
 /- [core::num::nonzero::NonZeroU32]
    Source: '/rustc/d59363ad0b6391b7fc5bbb02c9ccf9300eef3753/library/core/src/num/nonzero.rs', lines 50:12-50:33 -/
-axiom core.num.nonzero.NonZeroU32 : Type
+structure core.cell.Cell (T : Type) :=
+  id : Nat
 
-/- The state type used in the state-error monad -/
+def CellValue := (T:Type) × T
+
+/- The state type used in the state-error monad
+
+   TODO: we tried the following definition, but it makes State a Type 1, leading
+   to type errors later:
+
+     structure State :=
+       cells : AssocList Nat CellValue
+  -/
 axiom State : Type
-
