tests/fstar/misc/External.FunsExternal.fsti
@@ -6,20 +6,18 @@ include External.Types
 
 #set-options "--z3rlimit 50 --fuel 1 --ifuel 1"
 
-(** [core::mem::swap]:
-    Source: '/rustc/d59363ad0b6391b7fc5bbb02c9ccf9300eef3753/library/core/src/mem/mod.rs', lines 726:0-726:42
-    Name pattern: core::mem::swap *)
-val core_mem_swap (t : Type0) : t -> t -> state -> result (state & (t & t))
+(** [core::cell::{core::cell::Cell<T>#10}::get]:
+    Source: '/rustc/d59363ad0b6391b7fc5bbb02c9ccf9300eef3753/library/core/src/cell.rs', lines 497:4-497:26
+    Name pattern: core::cell::{core::cell::Cell<@T>}::get *)
+val core_cell_Cell_get
+  (t : Type0) (markerCopyInst : core_marker_Copy_t t) :
+  core_cell_Cell_t t -> state -> result (state & t)
 
-(** [core::num::nonzero::{core::num::nonzero::NonZeroU32#14}::new]:
-    Source: '/rustc/d59363ad0b6391b7fc5bbb02c9ccf9300eef3753/library/core/src/num/nonzero.rs', lines 79:16-79:57
-    Name pattern: core::num::nonzero::{core::num::nonzero::NonZeroU32}::new *)
-val core_num_nonzero_NonZeroU32_new
-  : u32 -> state -> result (state & (option core_num_nonzero_NonZeroU32_t))
-
-(** [core::option::{core::option::Option<T>}::unwrap]:
-    Source: '/rustc/d59363ad0b6391b7fc5bbb02c9ccf9300eef3753/library/core/src/option.rs', lines 932:4-932:34
-    Name pattern: core::option::{core::option::Option<@T>}::unwrap *)
-val core_option_Option_unwrap
-  (t : Type0) : option t -> state -> result (state & t)
+(** [core::cell::{core::cell::Cell<T>#11}::get_mut]:
+    Source: '/rustc/d59363ad0b6391b7fc5bbb02c9ccf9300eef3753/library/core/src/cell.rs', lines 574:4-574:39
+    Name pattern: core::cell::{core::cell::Cell<@T>}::get_mut *)
+val core_cell_Cell_get_mut
+  (t : Type0) :
+  core_cell_Cell_t t -> state -> result (state & (t & (t -> state -> result
+    (state & (core_cell_Cell_t t)))))
 
